Move alloc proof to separate file and clean up

src/goose_lang/my_stuff/alloc_proof.v
@@ -1,8 +1,53 @@
-From Perennial.goose_lang Require Import alloc.
-From Perennial.goose_lang.lib Require Import encoding.
+From Goose.github_com.mit_pdos.goose_nfsd Require Import alloc.
 From Perennial.program_proof Require Import proof_prelude.
 From Perennial.program_proof Require Import disk_lib.
-From Perennial.program_proof Require Import marshal_proof.
 
 Section proof.
 Context `{!heapG Σ}.
+
+Local Opaque struct_mapsto load_ty store_ty.
+
+(* Let's define what a valid allocator even looks like. *)
+
+Definition alloc_fields (l:loc) (next:u64) (bitmap:Slice.t): iProp Σ :=
+  l ↦[Alloc.S :: "next"] #next ∗
+  l ↦[Alloc.S :: "bitmap"] slice_val bitmap. (* casts Slice.t to a val (see slice.v) *)
+
+(* increment x mod n *)
+Definition mod_inc (x n: u64) : u64 :=
+  if (ge_dec (int.nat x + 1) (int.nat n)) then 0 else word.add x 1.
+
+Theorem incNext_spec stk E l next bitmap :
+  {{{ alloc_fields l next bitmap }}}
+    Alloc__incNext #l @stk; E
+  {{{ RET #(mod_inc next (8*int.nat bitmap.(Slice.sz)));
+        alloc_fields l (mod_inc next (8*int.nat bitmap.(Slice.sz))) bitmap }}}.
+
+Proof.
+  iIntros (Φ) "Halloc HΦ".
+  wp_call.
+  unfold alloc_fields in *.
+  iDestruct "Halloc" as "[H1 H2]".
+  wp_loadField. (* needed to split Halloc to make this work *)
+  wp_storeField.
+  wp_loadField.
+
+  wp_rec. (* this actually did something tiny *)
+
+  wp_loadField. (* why does this work now? *)
+
+  wp_pures.
+  wp_bind (If _ _ _).
+  wp_if_destruct.
+  (* this may be easier if we define mod_inc to fit the structure better. *)
+  - wp_storeField. wp_seq. wp_loadField. unfold mod_inc in *.
+    destruct (ge_dec (int.nat next + 1) (int.nat (8 * int.nat bitmap.(Slice.sz)))) eqn:Hinc2.
+    + iApply "HΦ". iFrame.
+    + admit.
+  - wp_seq. wp_loadField. unfold mod_inc in *.
+    destruct (ge_dec (int.nat next + 1) (int.nat (8 * int.nat bitmap.(Slice.sz)))) eqn:Hinc2.
+    + admit. (* contradiction here *)
+    + iApply "HΦ". iFrame.
+Admitted.
+
+End proof.
